Removal of UNITY/UNITYMisc, moving its theorems elsewhere. Conversion of UNITY/State to Isar format.;

src/ZF/UNITY/State.thy
@@ -9,27 +9,132 @@ Formalizes UNITY-program states using dependent types so that:
  - variables can be quantified over.
 *)
 
-State = UNITYMisc +
+header{*UNITY Program States*}
 
-consts var::i
-datatype var = Var("i:list(nat)")
-         type_intrs "[list_nat_into_univ]"
+theory State = Main:
+
+consts var :: i
+datatype var = Var("i \<in> list(nat)")
+  type_intros  nat_subset_univ [THEN list_subset_univ, THEN subsetD]
+
 consts
-  type_of :: i=>i
-  default_val :: i=>i
+  type_of :: "i=>i"
+  default_val :: "i=>i"
 
 constdefs
   state   :: i
-  "state == PROD x:var. cons(default_val(x), type_of(x))"
+   "state == \<Pi>x \<in> var. cons(default_val(x), type_of(x))"
+
   st0     :: i
-  "st0 == lam x:var. default_val(x)"
+   "st0 == \<lambda>x \<in> var. default_val(x)"
   
-  st_set  :: i =>o
+  st_set  :: "i=>o"
 (* To prevent typing conditions like `A<=state' from
    being used in combination with the rules `constrains_weaken', etc. *)
   "st_set(A) == A<=state"
 
-  st_compl :: i=>i
+  st_compl :: "i=>i"
   "st_compl(A) == state-A"
-  
+
+
+lemma st0_in_state [simp,TC]: "st0 \<in> state"
+by (simp add: state_def st0_def)
+
+lemma st_set_Collect [iff]: "st_set({x \<in> state. P(x)})"
+by (simp add: st_set_def, auto)
+
+lemma st_set_0 [iff]: "st_set(0)"
+by (simp add: st_set_def)
+
+lemma st_set_state [iff]: "st_set(state)"
+by (simp add: st_set_def)
+
+(* Union *)
+
+lemma st_set_Un_iff [iff]: "st_set(A Un B) <-> st_set(A) & st_set(B)"
+by (simp add: st_set_def, auto)
+
+lemma st_set_Union_iff [iff]: "st_set(Union(S)) <-> (\<forall>A \<in> S. st_set(A))"
+by (simp add: st_set_def, auto)
+
+(* Intersection *)
+
+lemma st_set_Int [intro!]: "st_set(A) | st_set(B) ==> st_set(A Int B)"
+by (simp add: st_set_def, auto)
+
+lemma st_set_Inter [intro!]: 
+   "(S=0) | (\<exists>A \<in> S. st_set(A)) ==> st_set(Inter(S))"
+apply (simp add: st_set_def Inter_def, auto)
+done
+
+(* Diff *)
+lemma st_set_DiffI [intro!]: "st_set(A) ==> st_set(A - B)"
+by (simp add: st_set_def, auto)
+
+lemma Collect_Int_state [simp]: "Collect(state,P) Int state = Collect(state,P)"
+by auto
+
+lemma state_Int_Collect [simp]: "state Int Collect(state,P) = Collect(state,P)"
+by auto
+
+
+(* Introduction and destruction rules for st_set *)
+
+lemma st_setI: "A <= state ==> st_set(A)"
+by (simp add: st_set_def)
+
+lemma st_setD: "st_set(A) ==> A<=state"
+by (simp add: st_set_def)
+
+lemma st_set_subset: "[| st_set(A); B<=A |] ==> st_set(B)"
+by (simp add: st_set_def, auto)
+
+
+lemma state_update_type: 
+     "[| s \<in> state; x \<in> var; y \<in> type_of(x) |] ==> s(x:=y):state"
+apply (simp add: state_def)
+apply (blast intro: update_type)
+done
+
+lemma st_set_compl [simp]: "st_set(st_compl(A))"
+by (simp add: st_compl_def, auto)
+
+lemma st_compl_iff [simp]: "x \<in> st_compl(A) <-> x \<in> state & x \<notin> A"
+by (simp add: st_compl_def)
+
+lemma st_compl_Collect [simp]:
+     "st_compl({s \<in> state. P(s)}) = {s \<in> state. ~P(s)}"
+by (simp add: st_compl_def, auto)
+
+(*For using "disjunction" (union over an index set) to eliminate a variable.*)
+lemma UN_conj_eq:
+     "\<forall>d\<in>D. f(d) \<in> A ==> (\<Union>k\<in>A. {d\<in>D. P(d) & f(d) = k}) = {d\<in>D. P(d)}"
+by blast
+
+
+ML
+{*
+val st_set_def = thm "st_set_def";
+val state_def = thm "state_def";
+
+val st0_in_state = thm "st0_in_state";
+val st_set_Collect = thm "st_set_Collect";
+val st_set_0 = thm "st_set_0";
+val st_set_state = thm "st_set_state";
+val st_set_Un_iff = thm "st_set_Un_iff";
+val st_set_Union_iff = thm "st_set_Union_iff";
+val st_set_Int = thm "st_set_Int";
+val st_set_Inter = thm "st_set_Inter";
+val st_set_DiffI = thm "st_set_DiffI";
+val Collect_Int_state = thm "Collect_Int_state";
+val state_Int_Collect = thm "state_Int_Collect";
+val st_setI = thm "st_setI";
+val st_setD = thm "st_setD";
+val st_set_subset = thm "st_set_subset";
+val state_update_type = thm "state_update_type";
+val st_set_compl = thm "st_set_compl";
+val st_compl_iff = thm "st_compl_iff";
+val st_compl_Collect = thm "st_compl_Collect";
+*}
+
 end
